1. Moment of Inertia ( $I, [\text{kg}\cdot\text{mÂ²}]$ ) - the sum of the products between the mass and distance from the rotational axis of every component of the system
	
	$$I = \sum_{i=1}^n m_ir_i^2$$
	
	**a) properties**
	 - the higher the moment of inertia, the more difficult it is to make a system rotate
	 - every body has infinitely many moments of inertia, since they are different for every access of rotation
	
	![Moment of Inertia](Resources/Moment%20of%20Inertia.jpg)
	
	**b) parallel axis theorem** - a simple relationship between the moment of inertia about an axis which is parallel to an axis going through the centre of mass
	
	$$I_{\text{P}} = I_{\text{cm}} + Md^2$$
	
	![Parallel Axis Theorem](Resources/Parallel%20Axis%20Theorem.jpg)
	
	Derivation:
	
	![Parallel Axis Theorem Proof](Resources/Parallel%20Axis%20Theorem%20Proof.jpg)
	
	Consider two axes parallel to the z-axis - one going through the centre of mass and another going through a point $P(a, b)$. The distance between the two axes is given by $d^2 = a^2 + b^2$.
	
	Take a mass element $m_i$ with coordinates $(x_i, y_i, z_i)$. 
	
	The moment of inertia around the centre-of-mass axis is then given by:
	
	$$I_{\text{cm}} = \sum_{i=1}^{n} m_i(x_i^2+y_i^2)$$
	
	The moment of inertia around the axis which goes through $P$ is given by:
	
	$$I_{\text{P}} = \sum_{i=1}^{n} m_i[(x_i-a)^2 + (y_i - b)]$$
	
	Expanding and rearranging...
	
	$$I_{\text{P}} = \sum_{i=1}^{n} m_i (x_i^2 + y_i^2) - 2a\sum_{i=1}^{n} m_ix_i - 2b\sum_{i=1}^{n} m_iy_i + (a^2 + b^2)\sum_{i=1}^{n} m_i$$
	
	The first term is just $I_{\text{cm}}$. From the definition of the centre of mass, the second and third terms are equal to $-2aMx_{\text{cm}}$ and $-2bMy_{\text{cm}}$, respectively, but these are both 0 on account that the centre of mass is at the origin of our chosen coordinate system. The last term is just the distance between the centre of mass times the total mass, which completes the proof.
	
	**c) moment of inertia** for rigid bodies with continuous mass distributions
	
	$$I = \int r^2\,dm = \int{r^2\rho}\,dV$$

2. Kinetic Energy
	
	**a) rotation only**
	
	$$K = \frac{1}{2}I\omega^2$$
	
	Derivation:
	
	The angular velocity for every component of the system is the same (otherwise the body wouldn't be rigid) and so the speed of the $i$-th component is given by
	
	$$v_i = r_i\omega$$
	
	Therefore, its kinetic energy is
	$$K_i = \frac{1}{2}m_ir_i^2\omega^2$$
	
	The total kinetic energy of the system is then
	
	$$K = \frac{1}{2} \left(\sum_{i=1}^n m_ir_i^2\right)\omega^2$$
	
	And we define the moment of inertia 
	to be
	
	$$I = \sum_{i=1}^n m_ir_i^2$$
	
	**b) combined translation and rotation**
	
	$$K = \frac{1}{2}mv_{\text{cm}}^2 + \frac{1}{2}I_{\text{cm}}\omega^2$$
	
	Derivation:
	
	![Kinetic Energy from Translation and Rotation](Resources/Kinetic%20Energy%20from%20Translation%20and%20Rotation.jpg)
	
	We are going to use the fact that the motion of any rigid body can be represented as a translation of the centre of mass and a rotation about it.
	
	The velocity of the $i$-th component relative to an inertial frame of reference, $\vec{v}_i$ is given by the velocity of the centre of mass $\vec{v}_{\text{cm}}$ plus the component's velocity relative to the centre of mass, $\vec{v}_i^{\prime}$, which is purely rotational:
	
	$$\vec{v}_i = \vec{v}_{\text{cm}} + \vec{v}_i^{\prime}$$
	
	The kinetic energy of this component in the inertial frame of reference is given by:
	
	$$K_i = \frac{1}{2}m_iv_i^2$$
	
	Now, $v_i^2$ is equal to $\vec{v}_i\cdot\vec{v}_i$ and so
	
	$$K_i = \frac{1}{2}m_i(\vec{v}_i\cdot\vec{v}_i)$$
	
	$$K_i = \frac{1}{2}m_i(\vec{v}_{\text{cm}} + \vec{v}_i^{\prime})\cdot(\vec{v}_{\text{cm}} + \vec{v}_i^{\prime}) = \frac{1}{2}m_i(\vec{v}_{\text{cm}}\cdot \vec{v}_{\text{cm}} + 2\vec{v}_{\text{cm}}\cdot\vec{v}_i^{\prime} + \vec{v}_i^{\prime}\cdot\vec{v}_i^{\prime}) = \frac{1}{2}m_i(v_{\text{cm}}^2 + 2\vec{v}_{\text{cm}}\cdot\vec{v}_i^{\prime} + v_i^{{\prime}^2})$$
	
	The total kinetic energy is
	
	$$K = \sum_{i=1}^n K_i = \frac{1}{2}\left(\sum_{i=1}^n m_i\right)v_{\text{cm}}^2 + \vec{v}_{\text{cm}}\cdot\left(\sum_{i=1}^n m_i\vec{v}_i^{\prime}\right) + \sum_{i=1}^n m_iv_i^{{\prime}^2}$$
	
	The first term is just $\frac{1}{2}M v_{\text{cm}}^2$.
	
	The second term is zero because $\sum m_i\vec{v_i}^{\prime}$ is $M$ times the velocity of the centre of mass *relative to the centre of mass* which is 0.
	
	The third term is just $\frac{1}{2}I_{\text{cm}}\omega^2$.

3. Work and Power
	
	**a) work**
	
	$$W = \int_{\theta_1}^{\theta_2} \tau\,d\theta$$
	
	Derivation:
	
	Suppose that a force acts on the rim of a pivoted disk. Only the tangential component of this force acts to change the rotation of the disk. For an infinitesimally small angle of rotation $d\theta$, a point on the rim moves $ds = R\,d\theta$. The infinitesimally small amount of work done by the force is then
	
	$$dW = F_{\text{tan}}\,ds = F_{\text{tan}}R\,d\theta = \tau\,d\theta$$
	
	The total work done for an angular displacement $\Delta \theta = \theta_2 - \theta_1$ is then given by the integral
	
	$$W = \int_{\theta_1}^{\theta_2} \tau\,d\theta$$
	
	Properties:
	- the work done by the net torque equals the total change in rotational kinetic energy
	
	**b) power**
	
	$$P = \tau\omega$$
	
	Derivation:
	
	$$dW = \tau\,d\theta$$
	
	$$\frac{dW}{dt} = \tau\frac{d\theta}{dt}$$
